More cleanup

src/example/elimstack/Code.v
@@ -9,11 +9,11 @@ Section ELIMSTACK.
   Context {state : Type}.
   Context {ident : ID}.
 
-  Definition push :
+  Definition push_loop :
     (* ktree (threadE void unit) (SCMem.val * SCMem.val) unit *)
     ktree (threadE ident state) (SCMem.val * SCMem.val) unit
     :=
-    fun '(s, val) => _ <- trigger Yield;; ITree.iter (fun (_ : unit) =>
+    fun '(s, val) => ITree.iter (fun (_ : unit) =>
       head <- (OMod.call (R:=SCMem.val) "load" s);;
       node <- (OMod.call (R:=SCMem.val) "alloc" 2);;
       _ <- (OMod.call (R:=unit) "store" (node,head));;
@@ -34,11 +34,19 @@ Section ELIMSTACK.
       if b then Ret (inl tt) else Ret (inr tt)
     ) tt.
 
-  Definition pop :
+  Definition push :
+    ktree (threadE ident state) (SCMem.val * SCMem.val) unit
+    :=
+    fun '(s, val) =>
+      _ <- trigger Yield;;
+      push_loop (s,val).
+
+  Definition pop_loop :
     (* ktree (threadE void unit) SCMem.val (option (SCMem.val) *)
     ktree (threadE ident state) SCMem.val (option (SCMem.val))
     :=
-    fun s => _ <- trigger Yield;; ITree.iter (fun (_ : unit) =>
+    fun s =>
+    ITree.iter (fun (_ : unit) =>
       head <- (OMod.call (R:=SCMem.val) "load" s);;
       is_null <- (OMod.call (R:=bool) "compare" (head, SCMem.val_null));;
       if is_null then Ret (inr None) else
@@ -63,6 +71,13 @@ Section ELIMSTACK.
           Ret (inl tt)
     ) tt.
 
+    Definition pop :
+    ktree (threadE ident state) SCMem.val (option SCMem.val)
+    :=
+    fun s =>
+      _ <- trigger Yield;;
+      pop_loop s.
+
     (** TODO : more rules for module composition. *)
     (* Definition omod : Mod.t := *)
     (*   Mod.mk *)
@@ -78,5 +93,65 @@ Section ELIMSTACK.
     (*     (SCMem.mod gvs) *)
     (* . *)
 
+    Lemma push_loop_red s val :
+      push_loop (s, val) =
+        head <- (OMod.call (R:=SCMem.val) "load" s);;
+        node <- (OMod.call (R:=SCMem.val) "alloc" 2);;
+        _ <- (OMod.call (R:=unit) "store" (node,head));;
+        _ <- (OMod.call (R:=unit) "store" (SCMem.val_add node 1, val));;
+        b <- (OMod.call (R:=bool) "cas" (s, head, node));;
+
+        if b then Ret tt else (
+
+        (* Attempt to exchange *)
+        _ <- (OMod.call (R:=unit) "store" (node,(0 : SCMem.val)));;
+        _ <- (OMod.call (R:=unit) "store" (SCMem.val_add s 1,node));;
+
+        (* Wait *)
+
+        (* Done waiting *)
+        _ <- (OMod.call (R:=unit) "store" (SCMem.val_add s 1,SCMem.val_null));;
+        b <- (OMod.call (R:=bool) "cas" (node, (0 : SCMem.val), (1 : SCMem.val)));;
+        if b then tau;; push_loop (s,val) else Ret tt
+        )
+      .
+    Proof.
+      unfold push_loop. etransitivity.
+      { apply unfold_iter_eq. }
+      grind.
+    Qed.
+
+    Lemma pop_loop_red s :
+      pop_loop s =
+        head <- (OMod.call (R:=SCMem.val) "load" s);;
+        is_null <- (OMod.call (R:=bool) "compare" (head, SCMem.val_null));;
+        if is_null then Ret None else
+
+        next <- (OMod.call (R:=SCMem.val) "load" head);;
+        b <- (OMod.call (R:=bool) "cas" (s, head, next));;
+
+        if b then
+          data <- (OMod.call (R:=SCMem.val) "load" (SCMem.val_add head 1));;
+          Ret (Some data)
+        else
+
+        offer <- (OMod.call (R:=SCMem.val) "load" (SCMem.val_add s 1));;
+
+        is_null <- (OMod.call (R:=bool) "compare" (offer, SCMem.val_null));;
+        if is_null then tau;; pop_loop s else
+          b <- (OMod.call (R:=bool) "cas" (offer, (0 : SCMem.val), (1 : SCMem.val)));;
+          if b then
+            data <- (OMod.call (R:=SCMem.val) "load" (SCMem.val_add offer 1));;
+            Ret (Some data)
+          else
+            tau;; pop_loop s
+      .
+    Proof.
+      unfold pop_loop. etransitivity.
+      { apply unfold_iter_eq. }
+      grind.
+    Qed.
+
+    Global Opaque push_loop pop_loop.
 End ELIMSTACK.
 End ElimStack.
