src/example/treiber/Code.v
@@ -10,12 +10,15 @@ Module TreiberStack.
     Context {ident : ID}.
 
     Definition push_loop :
-      ktree (threadE ident state) (SCMem.val * SCMem.val) (unit + unit)
-      := fun '(s, node) =>
+      ktree (threadE ident state) (SCMem.val * SCMem.val) unit
+      :=
+      fun '(s, node) =>
+      ITree.iter (fun (_ : unit) =>
         head <- (OMod.call (R:=SCMem.val) "load" s);;
         _ <- (OMod.call (R:=unit) "store" (node,head));;
         b <- (OMod.call (R:=bool) "cas" (s, head, node));;
-        if b then Ret (inr tt) else Ret (inl tt).
+        if b then Ret (inr tt) else Ret (inl tt)
+      ) tt.
 
     Definition push :
       (* ktree (threadE void unit) (SCMem.val * SCMem.val) unit *)
@@ -24,13 +27,14 @@ Module TreiberStack.
       fun '(s,val) =>
         node <- (OMod.call (R:=SCMem.val) "alloc" 2);;
         _ <- (OMod.call (R:=unit) "store" (SCMem.val_add node 1, val));;
-        _ <- ITree.iter (fun (_ : unit) => push_loop (s, node)) tt;;
+        _ <- push_loop (s, node);;
         trigger Yield.
 
     Definition pop_loop :
-      ktree (threadE ident state) SCMem.val (unit + option (SCMem.val))
+      ktree (threadE ident state) SCMem.val (option SCMem.val)
       :=
       fun s =>
+      ITree.iter (fun (_ : unit) =>
         head <- (OMod.call (R:=SCMem.val) "load" s);;
         is_null <- (OMod.call (R:=bool) "compare" (head, SCMem.val_null));;
         if is_null then Ret (inr None) else
@@ -41,7 +45,7 @@ Module TreiberStack.
           Ret (inr (Some data))
         else
           Ret (inl tt)
-        .
+      ) tt.
 
     Definition pop :
       (* ktree (threadE void unit) SCMem.val (option (SCMem.val) *)
@@ -49,7 +53,7 @@ Module TreiberStack.
       :=
       fun s =>
         _ <- trigger Yield;;
-        ITree.iter (fun (_ : unit) => pop_loop s) tt.
+        pop_loop s.
 
     (** TODO : more rules for module composition. *)
     (* Definition omod : Mod.t := *)
@@ -66,5 +70,36 @@ Module TreiberStack.
     (*     (SCMem.mod gvs) *)
     (* . *)
 
+  Lemma push_loop_red s node :
+    push_loop (s, node) =
+      head <- (OMod.call (R:=SCMem.val) "load" s);;
+      _ <- (OMod.call (R:=unit) "store" (node,head));;
+      b <- (OMod.call (R:=bool) "cas" (s, head, node));;
+      if b then Ret tt else tau;; push_loop (s,node).
+  Proof.
+    unfold push_loop. etransitivity.
+    { apply unfold_iter_eq. }
+    grind.
+  Qed.
+
+  Lemma pop_loop_red s :
+    pop_loop s =
+      head <- (OMod.call (R:=SCMem.val) "load" s);;
+      is_null <- (OMod.call (R:=bool) "compare" (head, SCMem.val_null));;
+      if is_null then Ret None else
+      next <- (OMod.call (R:=SCMem.val) "load" head);;
+      b <- (OMod.call (R:=bool) "cas" (s, head, next));;
+      if b then
+        data <- (OMod.call (R:=SCMem.val) "load" (SCMem.val_add head 1));;
+        Ret (Some data)
+      else
+        tau;; pop_loop s.
+  Proof.
+    unfold pop_loop. etransitivity.
+    { apply unfold_iter_eq. }
+    grind.
+  Qed.
+
+  Global Opaque push_loop pop_loop.
   End TREIBERSTACK.
 End TreiberStack.
